lean/privacy/subchannels/contiguous.lean
@@ -1,10 +1,10 @@
 import privacy.actions
 import privacy.utils
 
--- The k₁-s of subchannels for (c, k₀) form a contiguous range [0, k₁_bound).
+-- The k-s of subchannels for a given c form a contiguous range [0, k_bound).
 theorem subchannels_contiguous
-    {crypto: Crypto} (rm: ReachableMemory crypto) (c k₀) :
-    ∃ k₁_bound, ∀ k₁, (k₁ < k₁_bound) ↔ rm.m .SubchannelTokens [crypto.hash [c, k₀, k₁], 0] ≠ 0 := by
+    {crypto: Crypto} (rm: ReachableMemory crypto) (c: ℕ) :
+    ∃ k_bound, ∀ k, (k < k_bound) ↔ rm.m .SubchannelTokens [crypto.hash [c, k], 0] ≠ 0 := by
   revert rm
   apply ReachableMemory.induction
   case inv₀ => use 0; simp [ReachableMemory.m]
@@ -17,55 +17,55 @@ theorem subchannels_contiguous
     have info := open_subchannel_info crypto inp rm success
     rw [ReachableMemory.add_m, run_action, ←info.h_m']
 
-    obtain ⟨k₁_bound, h⟩ := h
+    obtain ⟨k_bound, h⟩ := h
 
-    by_cases h_is_same: c = inp.c ∧ k₀ = inp.k₀
+    by_cases h_is_same: c = inp.c
     case pos =>
-      use k₁_bound + 1
-      intro k₁
+      use k_bound + 1
+      intro k
 
-      have h_inp_k₁_not_small : ¬inp.k₁ < k₁_bound := by
+      have h_inp_k_not_small : ¬inp.k < k_bound := by
         by_contra h'
-        have := (h inp.k₁).1 h'
+        have := (h inp.k).1 h'
         simp only [h_is_same] at this
         have := info.old_token_was_zero
         contradiction
 
-      have h_inp_k₁_not_big : ¬inp.k₁ > k₁_bound := by
+      have h_inp_k_not_big : ¬inp.k > k_bound := by
         cases info.prev_subchannel_exists
         case inl h_prev => omega
         case inr h_prev =>
-          have := (h (inp.k₁ - 1)).2 (by
+          have := (h (inp.k - 1)).2 (by
             simp only [h_is_same]
             exact h_prev
           )
           omega
 
-      have h_k₁ : k₁_bound = inp.k₁ := by omega
+      have h_k : k_bound = inp.k := by omega
 
       have := info.memory_diff₁
-      by_cases h_k₁': k₁ = inp.k₁
+      by_cases h_k': k = inp.k
       case pos =>
-        rw [h_k₁, h_k₁', h_is_same.1, h_is_same.2, info.memory_diff₀]
+        rw [h_k, h_k', h_is_same, info.memory_diff₀]
         simp [info.r_ne_zero]
       case neg =>
-        have : crypto.hash [c, k₀, k₁] ≠ inp.subchannel_id crypto := by
+        have : crypto.hash [c, k] ≠ inp.subchannel_id crypto := by
           by_contra h'
           have := crypto.h_hash h'
           injections
           omega
         rw [info.no_change _ _ (by simp) (by simp [this]) (by simp)]
         constructor
-        · intro h₀; exact (h k₁).1 (by omega)
-        · intro h₀; have := (h k₁).2 h₀; omega
+        · intro h₀; exact (h k).1 (by omega)
+        · intro h₀; have := (h k).2 h₀; omega
     case neg =>
-      use k₁_bound
-      intro k₁
-      have : crypto.hash [c, k₀, k₁] ≠ inp.subchannel_id crypto := by
+      use k_bound
+      intro k
+      have : crypto.hash [c, k] ≠ inp.subchannel_id crypto := by
         by_contra h'
         have := crypto.h_hash h'
         injections
-        omega
+        contradiction
       rw [info.no_change _ _ (by simp) (by simp [this]) (by simp)]
-      exact h k₁
+      exact h k
   all_goals intro h success; try exact h
